Finished RemoveUpdates part of reduction proof

ironfleet/src/Dafny/Distributed/Concur/RemoveUpdates.i.dfy
@@ -2,6 +2,7 @@ include "Reduction.i.dfy"
 include "RefinementConvolution.i.dfy"
 include "SystemRefinement.i.dfy"
 include "ReductionPlan.i.dfy"
+include "MatchTreesToTrace.i.dfy"
 include "../Common/Collections/Maps.i.dfy"
 
 module RemoveUpdatesModule {
@@ -10,6 +11,7 @@ module RemoveUpdatesModule {
     import opened RefinementConvolutionModule
     import opened SystemRefinementModule
     import opened ReductionPlanModule
+    import opened MatchTreesToTraceModule
     import opened Collections__Maps_i
 
     function RemoveActorStatesFromSystemState(ls:SystemState) : SystemState
@@ -124,18 +126,196 @@ module RemoveUpdatesModule {
         }
     }
 
-    lemma {:axiom} lemma_ReductionOfBehaviorWithoutStates(
+    function RemoveLocalStateUpdates(trace:Trace) : Trace
+    {
+        if |trace| == 0 then
+            []
+        else if trace[0].action.UpdateLocalState? then
+            RemoveLocalStateUpdates(trace[1..])
+        else
+            [trace[0]] + RemoveLocalStateUpdates(trace[1..])
+    }
+
+    lemma lemma_IfNoLocalStateUpdatesThenRemoveLocalStateUpdatesIsIdentity(trace:Trace)
+        requires forall entry :: entry in trace ==> !entry.action.UpdateLocalState?;
+        ensures  trace == RemoveLocalStateUpdates(trace);
+    {
+    }
+
+    lemma lemma_GetPositionOfEntryInTraceWithoutLocalStateUpdates(trace:Trace, cur_pos:int) returns (new_pos:int)
+        requires 0 <= cur_pos < |trace|;
+        requires !trace[cur_pos].action.UpdateLocalState?;
+        ensures  0 <= new_pos < |RemoveLocalStateUpdates(trace)|;
+        ensures  RemoveLocalStateUpdates(trace)[new_pos] == trace[cur_pos];
+    {
+        if cur_pos == 0 {
+            new_pos := 0;
+            return;
+        }
+        if trace[0].action.UpdateLocalState? {
+            new_pos := lemma_GetPositionOfEntryInTraceWithoutLocalStateUpdates(trace[1..], cur_pos-1);
+        }
+        else {
+            var new_pos' := lemma_GetPositionOfEntryInTraceWithoutLocalStateUpdates(trace[1..], cur_pos-1);
+            new_pos := new_pos' + 1;
+        }
+    }
+
+    lemma lemma_GetPositionOfEntryInTraceBeforeRemovingLocalStateUpdates(trace:Trace, new_pos:int) returns (cur_pos:int)
+        requires 0 <= new_pos < |RemoveLocalStateUpdates(trace)|;
+        ensures  0 <= cur_pos < |trace|;
+        ensures  !trace[cur_pos].action.UpdateLocalState?;
+        ensures  RemoveLocalStateUpdates(trace)[new_pos] == trace[cur_pos];
+    {
+        if trace[0].action.UpdateLocalState? {
+            var cur_pos' := lemma_GetPositionOfEntryInTraceBeforeRemovingLocalStateUpdates(trace[1..], new_pos);
+            cur_pos := cur_pos' + 1;
+        }
+        else if new_pos == 0 {
+            cur_pos := 0;
+        }
+        else {
+            var cur_pos' := lemma_GetPositionOfEntryInTraceBeforeRemovingLocalStateUpdates(trace[1..], new_pos-1);
+            cur_pos := cur_pos' + 1;
+        }
+    }
+
+    lemma lemma_SkippingLocalStateUpdatePreservesRemoveLocalStateUpdates(
+        ltrace:Trace,
+        mtrace:Trace,
+        cur_pos:int
+        )
+        requires 0 <= cur_pos < |ltrace|;
+        requires ltrace[cur_pos].action.UpdateLocalState?;
+        requires |mtrace| == |ltrace| - 1;
+        requires forall i :: 0 <= i < |mtrace| ==> mtrace[i] == (if i < cur_pos then ltrace[i] else ltrace[i+1]);
+        ensures  RemoveLocalStateUpdates(ltrace) == RemoveLocalStateUpdates(mtrace);
+    {
+        if cur_pos == 0 {
+            assert mtrace == ltrace[1..];
+            assert RemoveLocalStateUpdates(ltrace) == RemoveLocalStateUpdates(ltrace[1..]);
+        }
+        else  {
+            lemma_SkippingLocalStateUpdatePreservesRemoveLocalStateUpdates(ltrace[1..], mtrace[1..], cur_pos - 1);
+        }
+    }
+
+    lemma lemma_RemoveLocalStateUpdatesMaintainsRestrictTraceToTrackedActions(trace:Trace)
+        ensures RestrictTraceToTrackedActions(trace) == RestrictTraceToTrackedActions(RemoveLocalStateUpdates(trace));
+    {
+        if |trace| == 0 {
+            return;
+        }
+
+        lemma_RemoveLocalStateUpdatesMaintainsRestrictTraceToTrackedActions(trace[1..]);
+    }
+        
+
+    lemma lemma_RemoveLocalStateUpdates(
         config:Config,
-        trace:Trace,
+        ltrace:Trace,
+        lb:SystemBehavior,
+        cur_pos:int
+        ) returns (
+        htrace:Trace,
+        hb:SystemBehavior
+        )
+        requires IsValidSystemTraceAndBehavior(config, ltrace, lb);
+        requires forall ls :: ls in lb ==> ls.states == map [];
+        requires 0 <= cur_pos <= |ltrace|;
+        requires forall i :: 0 <= i < cur_pos ==> !ltrace[i].action.UpdateLocalState?;
+        ensures  IsValidSystemTraceAndBehavior(config, htrace, hb);
+        ensures  SystemBehaviorRefinesSystemBehavior(lb, hb);
+        ensures  htrace == RemoveLocalStateUpdates(ltrace);
+        ensures  forall i :: 0 <= i < |htrace| ==> !htrace[i].action.UpdateLocalState?;
+        ensures  |hb| <= |lb|;
+        ensures  forall hs :: hs in hb ==> hs.states == map [];
+        decreases |ltrace| - cur_pos;
+    {
+        if cur_pos == |ltrace| {
+            htrace := ltrace;
+            hb := lb;
+            lemma_SystemBehaviorRefinesItself(lb);
+            lemma_IfNoLocalStateUpdatesThenRemoveLocalStateUpdatesIsIdentity(ltrace);
+            return;
+        }
+
+        if !ltrace[cur_pos].action.UpdateLocalState? {
+            htrace, hb := lemma_RemoveLocalStateUpdates(config, ltrace, lb, cur_pos + 1);
+            return;
+        }
+
+        var ls := lb[cur_pos];
+        var ls' := lb[cur_pos+1];
+        assert SystemNextEntry(ls, ls', ltrace[cur_pos]);
+        assert SystemNextUpdateLocalState(ls, ls', ltrace[cur_pos].actor);
+        assert ls' == ls;
+
+        var mtrace := ConvertMapToSeq(|ltrace|-1, map i | 0 <= i < |ltrace|-1 :: if i < cur_pos then ltrace[i] else ltrace[i+1]);
+        var mb := ConvertMapToSeq(|lb|-1, map i | 0 <= i < |lb|-1 :: if i <= cur_pos then lb[i] else lb[i+1]);
+        lemma_SkippingLocalStateUpdatePreservesRemoveLocalStateUpdates(ltrace, mtrace, cur_pos);
+        assert IsValidSystemTraceAndBehavior(config, mtrace, mb);
+
+        var relation := GetSystemSystemRefinementRelation();
+        var lm_map := ConvertMapToSeq(|lb|, map i | 0 <= i < |lb| :: if i <= cur_pos then RefinementRange(i, i) else RefinementRange(i-1, i-1));
+        forall i, j {:trigger RefinementPair(lb[i], mb[j]) in relation} | 0 <= i < |lb| && lm_map[i].first <= j <= lm_map[i].last
+            ensures RefinementPair(lb[i], mb[j]) in relation;
+        {
+            if i < cur_pos {
+                assert j == i;
+                assert lb[i] == mb[j];
+            }
+            else if i == cur_pos {
+                assert j == i;
+                assert lb[i] == ls == ls' == lb[i+1] == mb[j];
+            }
+            else {
+                assert j == i-1;
+                assert lb[i] == mb[j];
+            }
+            lemma_SystemStateCorrespondsToItself(lb[i]);
+        }
+
+        assert BehaviorRefinesBehaviorUsingRefinementMap(lb, mb, relation, lm_map);
+        assert SystemBehaviorRefinesSystemBehavior(lb, mb);
+
+        htrace, hb := lemma_RemoveLocalStateUpdates(config, mtrace, mb, cur_pos);
+        lemma_SystemSystemRefinementConvolutionPure(lb, mb, hb);
+    }
+
+    lemma lemma_ReductionOfBehaviorWithoutStates(
+        config:Config,
+        ltrace:Trace,
         lb:SystemBehavior,
         plan:ReductionPlan
         )
-        requires IsValidSystemTraceAndBehavior(config, trace, lb);
+        requires IsValidSystemTraceAndBehavior(config, ltrace, lb);
         requires IsValidReductionPlan(config, plan);
-        requires forall entry :: entry in trace ==> IsRealAction(entry.action);
+        requires forall entry :: entry in ltrace ==> IsRealAction(entry.action);
         requires forall actor :: actor in config.tracked_actors ==>
-                     RestrictTraceToTrackedActions(RestrictTraceToActor(trace, actor)) == GetEntries(plan[actor].trees);
+                     RestrictTraceToActor(RestrictTraceToTrackedActions(ltrace), actor) == GetEntries(plan[actor].trees);
         requires forall ls :: ls in lb ==> ls.states == map [];
         ensures  SystemBehaviorRefinesSpec(lb);
+    {
+        var htrace, hb := lemma_RemoveLocalStateUpdates(config, ltrace, lb, 0);
+        assert htrace == RemoveLocalStateUpdates(ltrace);
+
+        forall entry | entry in htrace
+            ensures IsRealAction(entry.action);
+        {
+            var hpos :| 0 <= hpos < |htrace| && entry == htrace[hpos];
+            var lpos := lemma_GetPositionOfEntryInTraceBeforeRemovingLocalStateUpdates(ltrace, hpos);
+        }
+
+        forall actor | actor in config.tracked_actors
+            ensures RestrictTraceToActor(RestrictTraceToTrackedActions(htrace), actor) == GetEntries(plan[actor].trees);
+        {
+            lemma_RemoveLocalStateUpdatesMaintainsRestrictTraceToTrackedActions(ltrace);
+            assert RestrictTraceToTrackedActions(htrace) == RestrictTraceToTrackedActions(ltrace);
+        }
+
+        lemma_ReductionOfBehaviorWithoutStatesOrUpdates(config, htrace, hb, plan);
+        lemma_SystemSpecRefinementConvolutionExtraPure(lb, hb);
+    }
 
 }
